bveq stuff

HMAC_spec_harvard.v
@@ -263,6 +263,1195 @@ Proof.
 Defined.
 *)
 
+
+Parameter bytes_bits_vector': forall (l : list Z) (n:nat) (bits: Bvector n), bool.
+
+Lemma bytes_bits_vector'_length l n bits:  
+   @bytes_bits_vector' l n bits = true -> n= (8 * length l)%nat.
+Admitted.
+
+
+(*
+Inductive bytes_bits_vector' (l : list Z) : Bvector (8 * length l) -> Prop :=
+  | eq_empty_v : forall (bits : Bvector (8 * length nil)),
+                   bytes_bits_vector' nil bits
+  (* TODO: might want to use Vector.nil bool? *)
+  | eq_cons_v : forall (bytes : list Z) (bits : Bvector (8 * length bytes))
+                       (byte : Z) (b0 b1 b2 b3 b4 b5 b6 b7 : bool),
+                  bytes_bits_vector' bytes bits ->
+                  convertByteBits byte [b0; b1; b2; b3; b4; b5; b6; b7] ->
+                  bytes_bits_vector' (byte :: bytes)
+                                     (* TODO: is this the right endianness? *)
+                                     (Vector.append [b0; b1; b2; b3; b4; b5; b6; b7] bits)
+*)
+
+
+Lemma list_cons_len {A : Type} :
+      forall (x : A) (xs : list A), length (x :: xs) = (1 + length xs)%nat.
+Proof. intros. reflexivity. Defined.
+
+Lemma mul_dist : forall (n m : nat), (n * (1 + m))%nat = (n + n * m)%nat.
+Proof.
+  intros. simpl.
+  rewrite -> mult_succ_r. rewrite -> plus_comm. reflexivity.
+Defined.
+
+Fixpoint squash_list_vector
+         (bits_list : list (Bvector 8)) : Bvector (8 * length bits_list).
+Proof.
+  destruct bits_list.
+    apply (Vector.nil bool).
+    rewrite -> list_cons_len.
+    rewrite -> mul_dist.
+    (* TODO watch out for endianness *)
+  apply (Vector.append b0 (squash_list_vector bits_list)).
+Defined.  
+
+SearchAbout Vector.cons.
+Check Vector.cons.
+Check Vector.cons bool true 1 [false].
+
+(* TODO: how to write a better dependent pattern match? doesn't use the equality of their len
+writing it as a proof and destructing n or b1/b2 doesn't work
+*)
+Fixpoint bvector_eq (n : nat) (m : nat) (b1 : Bvector n) (b2 : Bvector m) : bool :=
+  match b1, b2 with             (*  match n as n0 return (Bvector n0) with *)
+    | Vector.nil, Vector.nil => true
+    | Vector.cons x1 _ xs1, Vector.cons x2 _ xs2 =>
+      eqb x1 x2 && bvector_eq xs1 xs2
+    | _, _ => false                (* not possible *)
+  end.
+
+ 
+Definition bveqF := 
+fix bveqF (n : nat) (b1 b2 : Bvector n) {struct n} : bool :=
+  match n as n0 return (Bvector n0 -> Bvector n0 -> bool) with
+  | 0%nat => fun _ _ : Bvector 0 => true
+  | S n0 =>
+      fun b3 b4 : Bvector (S n0) =>
+      eqb (Vector.hd b3) (Vector.hd b4) &&
+      bveqF n0 (Vector.tl b3) (Vector.tl b4)
+  end b1 b2.
+
+Fixpoint bveq (n:nat) (b1 b2:Bvector n): bool.
+  destruct n; intros. apply true. remember (S n) as m.
+destruct b1. inversion Heqm. inversion Heqm. subst.  inversion b2. subst. 
+  apply (eqb h h0 && bveq _ b1 H0).
+(*  apply (eqb (Vector.hd b1) (Vector.hd b2) && (bveq _ (Vector.tl b1) (Vector.tl b2))).*)
+Defined.
+Print bveq.
+
+Definition bveq1 (n:nat) (b1 b2:Bvector n): bool.
+  induction n; intros. apply true.
+  apply (eqb (Vector.hd b1) (Vector.hd b2) && (IHn (Vector.tl b1) (Vector.tl b2))).
+Defined.
+
+Definition bveqD := 
+fun (n : nat) (b1 b2 : Bvector n) =>
+nat_rec (fun n0 : nat => Bvector n0 -> Bvector n0 -> bool)
+  (fun _ _ : Bvector 0 => true)
+  (fun (n0 : nat) (IHn : Bvector n0 -> Bvector n0 -> bool)
+     (b3 b4 : Bvector (S n0)) =>
+   eqb (Vector.hd b3) (Vector.hd b4) && IHn (Vector.tl b3) (Vector.tl b4)) n
+  b1 b2.
+
+
+Eval compute in (bveqD [true; true; false] [true; true; false]).
+
+(*
+Fixpoint bvector_eq (n : nat) (b1 : Bvector n) (b2 : Bvector n) : bool :=
+  match b1, b2 with             (*  match n as n0 return (Bvector n0) with *)
+    | Vector.nil, Vector.nil => true
+    | Vector.cons x1 _ xs1, Vector.cons x2 _ xs2 =>
+      eqb x1 x2 && bvector_eq xs1 xs2
+    | _, _ => false                (* not possible *)
+  end.
+  *)
+(* TODO watch out for endianness *)
+Search Bvector.
+Inductive bytes_bits_vector_comp1: forall n
+         (bytes : list Z) (bits : Bvector n), Prop:=
+bvv_nil: bytes_bits_vector_comp1 nil []
+| bvv_cons: forall n bytes1 bits1 
+                       (bt : Z) (b0 b1 b2 b3 b4 b5 b6 b7 : bool),
+                  @bytes_bits_vector_comp1 n bytes1 bits1 ->
+                  convertByteBits bt [b0; b1; b2; b3; b4; b5; b6; b7] ->
+                  @bytes_bits_vector_comp1 (8 + n) (bt :: bytes1)
+                                     (* TODO: is this the right endianness? *)
+                                     (Vector.append [b0; b1; b2; b3; b4; b5; b6; b7] bits1).
+(*
+Proof.
+  remember (map byte_to_bits bytes) as bits_list_vector.
+  remember (squash_list_vector bits_list_vector) as bvector.
+  assert (len_eq: length bytes = length bits_list_vector).
+    rewrite -> Heqbits_list_vector.
+    rewrite -> list_length_map.
+    reflexivity.
+  rewrite -> len_eq in bits.
+  apply (bveqD bvector bits).
+Defined.
+
+Fixpoint bytes_bits_vector_comp
+         (bytes : list Z) n (bits : Bvector n) : bool.
+Proof.
+  remember (map byte_to_bits bytes) as bits_list_vector.
+  remember (squash_list_vector bits_list_vector) as bvector.
+  assert (len_eq: length bytes = length bits_list_vector).
+    rewrite -> Heqbits_list_vector.
+    rewrite -> list_length_map.
+    reflexivity.
+  rewrite -> len_eq in bits.
+  apply (bveqD bvector bits).
+Defined.
+
+Print bytes_bits_vector_comp.
+
+ Eval compute in
+    bytes_bits_vector_comp (0 :: nil) [true; true; true; true; true; true; true; true]. 
+*)
+(* TODO watch out for endianness *)
+Definition bytes_bits_vector_comp'
+         (bytes : list Z) (bits : Bvector (8 * length bytes)) : bool.
+Proof.
+  remember (map byte_to_bits bytes) as bits_list_vector.
+  remember (squash_list_vector bits_list_vector) as bvector.
+  assert (len_eq: length bytes = length bits_list_vector).
+    rewrite -> Heqbits_list_vector.
+    rewrite -> list_length_map.
+    reflexivity.
+  rewrite -> len_eq in bits.
+  apply (bvector_eq bvector bits).
+Defined.
+
+Print bytes_bits_vector_comp'.
+(* Seems hard to use in a proof... *)
+
+(* TODO: generates 20k-line expr *)
+ Eval compute in
+    bytes_bits_vector_comp' (0 :: nil) [true; true; true; true; true; true; true; true]. 
+  
+
+(* TODO: compare to rel1. How do dependent types and inductive props work? *)
+
+Check bytes_bits_vector.
+Check HMAC_SHA256.HMAC.         (* ? *)
+Check HMAC.
+(* HMAC
+     : forall c p : nat,
+       (Bvector c -> Bvector (b c p) -> Bvector c) ->   // compression function h
+       Bvector c ->                          // iv, h's initialization vector
+       (Blist -> list (Bvector (b c p))) ->  // splitAndPad (e.g. generate_and_pad)
+       Bvector p ->                          // fpad, constant-length padding
+       Bvector (b c p) ->                    // opad
+       Bvector (b c p) ->                    // ipad
+
+^ Note: this has to do with the internals of SHA256 and HMAC too
+SHA's compression function, iv, generate_and_pad (with block vectors),
+HMAC's key padding function, HMAC's opad and ipad.
+How to convert?
+
+       Bvector (b c p) -> Blist -> Bvector c        // key, message, outputted hash
+
+k is of length b
+b = block size
+c = output size
+p = padding = b - c
+
+why pad the key? why not just let it be size b?
+ *)
+
+(* ----------------------------------------- Theorem and parameters *)
+
+(* want Bvector b = 512 bits *)
+Print Byte.int.
+Print Byte.repr.
+Check Byte.unsigned.
+Check HMAC_SHA256.sixtyfour.
+
+Definition opad_test := 
+     bytes_to_bits
+                     (map Byte.unsigned (HMAC_SHA256.sixtyfour (Byte.repr 52))).
+Check opad_test. 
+(* Definition ipad_test := bytes_to_bits
+                     (map Byte.unsigned (HMAC_SHA256.sixtyfour HMAC_SHA256.Ipad)). *)
+
+(*
+TODO: 8/20/14
+
+Key is not being padded? Need to assume the padded key is of length b
+Email Adam about fpad: it's not used to pad the key
+Figure out what parameters are
+Fill in the relations
+
+Byte to bits: computational vs. prop
+  bytes_bits_vector: problem
+  bytes_to_bits: 2 problems
+  still need the computational version for opad?
+
+Modify the theorem:
+ parametrize C HMAC by OPAD and IPAD + they need to be different in at least one bit
+   (email adam: does he use this in his proof?)
+
+Now, write individual functions and prove them equivalent? they have different types
+Still abstract: sha_h, sha_splitandpad, fpad?
+
+Figure out what lemmas to prove (Look in HMAC_Lemmas)
+
+Lennart: update spec to take ipad and opad as parameters
+ *)
+Check HMAC.
+
+(* ------------------------------------- *)
+Module Equiv.
+
+Definition c:nat := (SHA256_.DigestLength * 8)%nat.
+(*Variable p:nat.
+Locate HMAC.
+Check @HMAC. Check @sha_h.
+Check (@HMAC _ p (@sha_h _ p plus) sha_iv (sha_splitandpad_vector p) (fpad p)). 
+Check (HMAC (sha_h p plus) sha_iv).
+*)
+Definition p:=(32 * 8)%nat.
+
+Parameter sha_iv : Bvector (SHA256_.DigestLength * 8).
+
+(* Definition sha_h : list Z -> list Z := SHA256_.Hash. *)
+(* TODO: c = 32, p = 32 *)
+Parameter sha_h : Bvector c -> Bvector (c + p) -> Bvector c.
+
+(* corresponds to block size. b = plus *)
+
+(* TODO: email adam about fpad: it's not padding the key *)
+
+(*  "Blist -> list (Bvector (b SHA256_.DigestLength c))" *)
+Parameter sha_splitandpad_vector :
+  Blist -> list (Bvector (SHA256_.DigestLength * 8 + p)).
+
+Parameter fpad : Bvector p.
+
+(* Define opad, define ipad, pass converted ipad/opad to respective hmacs *)
+
+(* Is this the theorem we want? Is it useful for the rest of the proofs?
+Should it be more abstract? *)
+
+(* TODO: opad <> ipad? *)
+(* TODO fill this in *)
+(* relies on bytes_bits_vector' too *)
+Parameter bytes_bits_conv_vector' : byte -> Bvector (plus c p) -> Prop.
+(* Does something like: 
+bytes_bits_vector' (map Byte.unsigned (sixtyfour opad)) OPAD *)
+
+(*  (let (k_Out, k_In) :=
+                       splitVector (b 256 256) (b 256 256)
+                         (Vector.append (BVxor (b 256 256) K OP)
+                            (BVxor (b 256 256) K IP)) in 
+Possibly try n = m -> splitVector n m...
+*)
+
+SearchAbout Bvector.
+(* SearchAbout Vector. *)
+
+Lemma empty_vector : forall (v : Bvector 0),
+                       v = [].
+Proof.
+  intros v.
+  (* destruct v. *)
+
+Admitted.
+
+Lemma split_append_id : forall (len : nat) (v1 v2 : Bvector len),
+                          splitVector len len (Vector.append v1 v2) = (v1, v2).
+Proof.
+  induction len; intros v1 v2.
+  (* Case len = 0 *)
+    (* simpl. rewrite -> empty_vector. *)
+
+
+    Admitted.
+
+
+(* TODO: 10/25/14
+- figure out old and new fpad (email adam) **
+- add lemma for xor **
+- fill in parameters: sha_h, sha_iv, sha_splitandpad_vector, fpad **
+- figure out how to get split lemmas to work
+- check bytes_bits_vector' fixpoint
+   - get it to to work with theorem **
+   - see if induction works with it
+   - write bytes_bits_conv_vector 
+- step through theorem
+  - figure out how to use relations in theorem
+
+ *)
+Theorem HMAC_spec_equiv : forall
+                            (k m h : list Z)
+                            (K : Bvector (plus c p)) (M : Blist) (H : Bvector c)
+                            (op ip : byte) (OP IP : Bvector (plus c p)),
+  ((length k) * 8)%nat = b c p ->
+  bytes_bits_vector_wrong k K ->
+  (* 1. not separating c and p 2. inductive prop / dep types? 3. computation / dep types?
+     bytes_bits_vector' k K vs. bytes_to_bits k = K <- can't prove lens equal?*)
+  bytes_bits_lists m M ->
+  bytes_bits_conv_vector' op OP ->
+  bytes_bits_conv_vector' ip IP ->
+  HMAC sha_h sha_iv sha_splitandpad_vector fpad OP IP K M = H ->
+  HMAC_SHA256.HMAC op ip m k = h -> (* m k, not k m *)
+  bytes_bits_vector_wrong h H.
+Proof.  
+  intros k m h K M H op ip OP IP.
+  intros padded_key_len padded_keys_eq msgs_eq ops_eq ips_eq.
+  intros HMAC_abstract HMAC_concrete.
+  unfold p,c, b in *.
+  simpl in *.
+
+  unfold HMAC in *.
+  unfold HMAC_SHA256.HMAC in *.
+
+  unfold HMAC_2K in *. unfold GHMAC_2K in *. (* unfold splitVector in *. *)
+  (* Still abstract: sha_h, sha_splitandpad_vector, fpad,
+     bytes_bits_vector', bytes_bits_conv_vector' *)
+  rewrite -> split_append_id in HMAC_abstract. (* wow! *)
+
+  unfold HMAC_SHA256.OUTER in *. unfold HMAC_SHA256.INNER in *.
+    unfold HMAC_SHA256.outerArg in *. unfold HMAC_SHA256.innerArg in *.
+    unfold HMAC_SHA256.mkArgZ in *. unfold HMAC_SHA256.mkArg in *.
+
+  unfold BVxor in *. unfold xorb in *. (* unfold Vector.map2 in *. *)
+  unfold Byte.xor in *. (* unfold Z.lxor in *. *)
+
+    (* Lemma:
+
+BVxor (b 256 256) K OP = Vector.map2 xorb K OP (can unfold xorb) 
+     ~
+                          (map
+                          (fun p0 : byte * byte => Byte.xor (fst p0) (snd p0))
+                          (combine (map Byte.repr (HMAC_SHA256.mkKey k))
+                             (HMAC_SHA256.sixtyfour ip)))
+
+plus i probably want a meta-lemma for composition of relations
+r1 x X -> r2 y Y -> f x y ~ F X Y
+
+figure out how to approach proof: 4-way induction sounds painful
+
+ *)
+
+    
+  rewrite <- HMAC_abstract.
+  rewrite <- HMAC_concrete.
+
+  
+  
+  induction msgs_eq.
+
+
+Abort.
+=======
+Set Implicit Arguments.
+
+Require Import Bvector.
+Require Import List.
+Require Import Arith.
+
+Require Import HMAC_functional_prog.
+Require Import Integers.
+Require Import Coqlib.
+
+(* Require Import List. Import ListNotations. *)
+
+Definition Blist := list bool.
+
+Fixpoint splitVector (A : Set) (n m : nat) :
+  Vector.t A (n + m) -> (Vector.t A n * Vector.t A m) :=
+  match n with
+    | 0%nat => 
+      fun (v : Vector.t A (O + m)) => (@Vector.nil A, v) (* why the function? TODO *)
+    | S n' => 
+      fun (v : Vector.t A (S n' + m)) => 
+        let (v1, v2) := splitVector _ _ (Vector.tl v) in
+          (Vector.cons _ (Vector.hd v) _ v1, v2)
+  end.
+
+Eval compute in splitVector 1 2 [true; true; true].
+
+Section HMAC.
+
+SearchAbout Bvector.
+Print Bvector.
+Check Bvector 10.
+Check [true]. 
+Print Vector.
+
+(* b = block size
+   c = digest (output) size
+   p = padding = b - c (fixed) *)
+  Variable c p : nat.
+  Definition b := (c + p)%nat.
+  
+  (* The compression function *)
+  Variable h : Bvector c -> Bvector b -> Bvector c.
+  (* The initialization vector is part of the spec of the hash function. *)
+  Variable iv : Bvector c.
+  (* The iteration of the compression function gives a keyed hash function on lists of words. *)
+  Definition h_star k (m : list (Bvector b)) :=
+    fold_left h m k.
+  (* The composition of the keyed hash function with the IV gives a hash function on lists of words. *)
+  Definition hash_words := h_star iv.
+
+  (* TODO check how this corresponds to SHA
+     Seems that h = SHA compression function
+     hash_words with SHA's iv is SHA
+   *)
+  Check hash_words.
+  Check h_star.
+
+  Variable splitAndPad : Blist -> list (Bvector b).
+
+  (* TODO examine this hypothesis, prove that MD lemmas imply it *)
+  Hypothesis splitAndPad_1_1 : 
+    forall b1 b2,
+      splitAndPad b1 = splitAndPad b2 ->
+      b1 = b2.
+  
+  (* constant-length padding. *)
+  Variable fpad : Bvector p.
+
+  Definition app_fpad (x : Bvector c) : Bvector b :=
+    (Vector.append x fpad).
+  Definition h_star_pad k x :=
+    app_fpad (h_star k x).
+
+  Definition GNMAC k m :=
+    let (k_Out, k_In) := splitVector c c k in
+    h k_Out (app_fpad (h_star k_In m)).
+
+  (* The "two-key" version of GHMAC and HMAC. *)
+  (* Concatenate (K xor opad) and (K xor ipad) *)
+  Definition GHMAC_2K (k : Bvector (b + b)) m :=
+    let (k_Out, k_In) := splitVector b b k in (* concat earlier, then split *)
+      let h_in := (hash_words (k_In :: m)) in 
+        hash_words (k_Out :: (app_fpad h_in) :: nil).
+  
+  Definition HMAC_2K (k : Bvector (b + b)) (m : Blist) :=
+    GHMAC_2K k (splitAndPad m).
+
+Check HMAC_2K.
+(* HMAC_2K
+     : Bvector (b + b) -> Blist -> Bvector c *)
+
+(* opad and ipad are constants defined in the HMAC spec. *)
+Variable opad ipad : Bvector b.
+Definition GHMAC (k : Bvector b) :=
+  GHMAC_2K (Vector.append (BVxor _ k opad) (BVxor _ k ipad)).
+
+Print BVxor.
+
+
+Definition HMAC (k : Bvector b) :=
+  HMAC_2K (Vector.append (BVxor _ k opad) (BVxor _ k ipad)).
+
+Check HMAC.                     (*  : Bvector b -> Blist -> Bvector c *)
+
+End HMAC.
+
+(* ----------------------------------------------------------- Theorem definitions *)
+
+Check HMAC_SHA256.HMAC.            (* list Z -> list Z -> list Z *)
+
+  (* Bvector is little-endian (least significant bit at head; list Z are just translated
+from the string (ascii -> nat -> Z); but Int are packed big-endian (with 4 Z -> 1 Int)
+
+each Z is one byte (8 bits) *)
+
+(* TODO: add isbyteZ (from SHA256.v), 0 <= i <= 256 *)
+
+(* *************** byte/bit computational *)
+
+(* TODO: finish this
+
+The term "Vector.append (iterate n' num_new) [bool_digit]" has type
+ "Vector.t bool (n' + 1)" while it is expected to have type 
+"Bvector (S n')".
+
+Function with proof of equivalence? see hash_blocks  *)
+
+(*
+Fixpoint iterate (n : nat) (byte : nat) : Bvector n :=
+  match n as x return Bvector x with
+    | O => Vector.nil bool
+    | S n' =>
+      let byte_subtract := (byte - NPeano.pow 2 n')%nat in
+      let bool_digit := negb (leb byte_subtract 0) in
+      let num_new := if bool_digit then byte_subtract else byte in
+      Vector.append (iterate n' num_new) [bool_digit] (* could reverse instead *)
+  end.
+
+*)
+
+Lemma add_1_r_S : forall (n : nat), (n + 1)%nat = S n.
+Proof.
+  induction n.
+    reflexivity.
+    simpl. rewrite -> IHn. reflexivity.
+Defined.
+
+(* TODO step through this *)
+Locate leb. Check negb.
+(* little-endian *)
+Fixpoint iterate (n : nat) (byte : nat) : Bvector n.
+Proof.
+  destruct n.
+     apply (Vector.nil bool).
+  remember ((byte - NPeano.pow 2 n)%nat) as byte_subtract.
+  remember (negb (leb byte_subtract 0)) as bool_digit. (* changed from leb: gt now *)
+  remember (if bool_digit then byte_subtract else byte) as num_new.
+  rewrite <- add_1_r_S.
+  apply (Vector.append (iterate n num_new) [bool_digit]). (* n' *)
+Defined.
+
+Print iterate.
+Eval compute in iterate 1 255.
+Check eq_rec. Print eq_rec. Print eq_rect. Check eq_rect.
+Print NPeano.Nat.add_1_r.
+
+(* TODO: fix the latter + 1 *)
+Fixpoint byte_to_bits (byte : Z) : Bvector 8 :=
+  let max_pow_two := 7%nat in
+  iterate (max_pow_two + 1) (nat_of_Z byte + 1).
+
+  Print add_1_r_S.
+Eval compute in iterate 8 2.
+Eval compute in byte_to_bits 0.
+Eval compute in byte_to_bits 1.
+Eval compute in byte_to_bits 2.
+
+Eval compute in byte_to_bits 127.
+Eval compute in byte_to_bits 128.
+Eval compute in byte_to_bits 129.
+Eval compute in byte_to_bits 200.
+Eval compute in byte_to_bits 255. 
+Eval compute in byte_to_bits 256. (* not valid *)
+
+(* Parameter byte_to_bits : Z -> Bvector 8. *)
+
+(* Or: concatMap byte_to_bit bytes *)
+Check Bvector.
+SearchAbout Bvector.
+Print Vector.t.
+
+(* how to prove that it's length bytes * 8? *)
+(* list of bytes? (type) *)
+Fixpoint bytes_to_bits (bytes : list Z) : Bvector (length bytes * 8) :=
+  match bytes as x return Bvector (length x * 8) with (* CPDT *)
+    | nil => Vector.nil bool
+    | x :: xs => Vector.append (byte_to_bits x) (bytes_to_bits xs)
+  end.
+
+
+
+(* ************* inductive defs *)
+  
+SearchAbout Bvector.
+
+Definition asZ (x : bool) : Z := if x then 1 else 0.
+
+(* TODO: maybe prefer b : byte, with Byte.repr? *)
+Definition convertByteBits (b : Z) (B : Bvector 8) : Prop :=
+  exists (b0 b1 b2 b3 b4 b5 b6 b7 : bool),
+   B = [b0; b1; b2; b3; b4; b5; b6; b7] /\
+   b =  (1 * (asZ b0) + 2 * (asZ b1) + 4 * (asZ b2) + 8 * (asZ b3)
+         + 16 * (asZ b4) + 32 * (asZ b5) + 64 * (asZ b6) + 128 * (asZ b7)).
+
+(* *** *)
+
+(* relationship between a list Z (of bytes) and a Bvector of size (c + p):
+toBvector (bytes_to_bits k) = K?
+
+This definition is not easy to use; replaced with bytes_bits_vector' in theorem
+ *)
+Inductive bytes_bits_vector (c p : nat) (k : list Z) : Bvector (plus c p) -> Prop :=
+  | test_n : forall (K : Bvector (plus c p)),
+               bytes_bits_vector c p k K (* TODO *)
+.
+
+(* relating list Z to Blist
+bytes_to_bits m = length M
+
+TODO: big-endian, little-endian?
+*)
+Inductive bytes_bits_lists : list Z -> Blist -> Prop :=
+  | eq_empty : bytes_bits_lists nil nil
+  | eq_cons : forall (bytes : list Z) (bits : Blist)
+                     (byte : Z) (b0 b1 b2 b3 b4 b5 b6 b7 : bool),
+                bytes_bits_lists bytes bits ->
+                convertByteBits byte [b0; b1; b2; b3; b4; b5; b6; b7] ->
+                bytes_bits_lists (byte :: bytes)
+                                (b0 :: b1 :: b2 :: b3 :: b4 :: b5 :: b6 :: b7 :: bits)
+.
+
+(* the hashes are "the same": list Z vs Bvector c
+
+toBvector (bytes_to_bits h) = H
+this is *almost* the same as bytes_bits_vector, except just c, not c + p
+ *)
+(* note: need to name c in order to use in Bvector c -- but then need to use names *)
+Inductive bytes_bits_vector_wrong (len : nat) (bytes : list Z) (bits : Bvector len) : Prop :=
+  | eq_empty_v' : bytes = nil -> len = 0%nat -> bytes_bits_vector_wrong bytes bits
+  | eq_cons_v' : bytes_bits_vector_wrong bytes bits.
+
+(*
+Fixpoint iterate (n : nat) (byte : nat) : Bvector n.
+Proof.
+  destruct n.
+     apply (Vector.nil bool).
+  remember ((byte - NPeano.pow 2 n)%nat) as byte_subtract.
+  remember (negb (leb byte_subtract 0)) as bool_digit. (* changed from leb: gt now *)
+  remember (if bool_digit then byte_subtract else byte) as num_new.
+  rewrite <- add_1_r_S.
+  apply (Vector.append (iterate n num_new) [bool_digit]). (* n' *)
+Defined.
+*)
+
+(*
+Inductive bytes_bits_vector' (l : list Z) : Bvector (8 * length l) -> Prop :=
+  | eq_empty_v : forall (bits : Bvector (8 * length nil)),
+                   bytes_bits_vector' nil bits
+  (* TODO: might want to use Vector.nil bool? *)
+  | eq_cons_v : forall (bytes : list Z) (bits : Bvector (8 * length bytes))
+                       (byte : Z) (b0 b1 b2 b3 b4 b5 b6 b7 : bool),
+                  bytes_bits_vector' bytes bits ->
+                  convertByteBits byte [b0; b1; b2; b3; b4; b5; b6; b7] ->
+                  bytes_bits_vector' (byte :: bytes)
+                                     (* TODO: is this the right endianness? *)
+                                     (Vector.append [b0; b1; b2; b3; b4; b5; b6; b7] bits)
+.
+*)
+
+Lemma list_cons_len {A : Type} :
+      forall (x : A) (xs : list A), length (x :: xs) = (1 + length xs)%nat.
+Proof. intros. reflexivity. Defined.
+
+Lemma mul_dist : forall (n m : nat), (n * (1 + m))%nat = (n + n * m)%nat.
+Proof.
+  intros. simpl.
+  rewrite -> mult_succ_r. rewrite -> plus_comm. reflexivity.
+Defined.
+
+Print mult_succ_r.
+Print plus_comm.
+
+Fixpoint squash_list_vector
+         (bits_list : list (Bvector 8)) : Bvector (8 * length bits_list).
+Proof.
+  destruct bits_list.
+    apply (Vector.nil bool).
+    rewrite -> list_cons_len.
+    rewrite -> mul_dist.
+    (* TODO watch out for endianness *)
+  apply (Vector.append b0 (squash_list_vector bits_list)).
+Defined.  
+
+SearchAbout Vector.cons.
+Check Vector.cons.
+Check Vector.cons bool true 1 [false].
+
+(* TODO: how to write a better dependent pattern match? doesn't use the equality of their len
+writing it as a proof and destructing n or b1/b2 doesn't work
+*)
+Fixpoint bvector_eq (n : nat) (m : nat) (b1 : Bvector n) (b2 : Bvector m) : bool :=
+  match b1, b2 with             (*  match n as n0 return (Bvector n0) with *)
+    | Vector.nil, Vector.nil => true
+    | Vector.cons x1 _ xs1, Vector.cons x2 _ xs2 =>
+      eqb x1 x2 && bvector_eq xs1 xs2
+    | _, _ => false                (* not possible *)
+  end.
+  
+(* TODO watch out for endianness *)
+  
+Definition bytes_bits_vector_comp
+         (n : nat) (bytes : list Z) (bits : Bvector n) : bool.
+Proof.
+  remember (map byte_to_bits bytes) as bits_list_vector.
+  remember (squash_list_vector bits_list_vector) as bvector.
+  assert (len_eq: length bytes = length bits_list_vector).
+    rewrite -> Heqbits_list_vector.
+    rewrite -> list_length_map.
+    reflexivity.
+  (* rewrite -> len_eq in bits. *)
+  apply (bvector_eq bvector bits).
+Defined.
+
+Print bytes_bits_vector_comp.
+(* Seems hard to use in a proof... *)
+
+(* TODO: get this to be required *)
+Eval compute in
+    bytes_bits_vector_comp (0 :: nil) [true; true; true; true; true; true; true; true].
+
+Lemma bytes_bits_vector_comp_len : forall (n : nat) (bytes : list Z) (bits : Bvector n),
+                                     bytes_bits_vector_comp bytes bits = true
+                                     -> n = (8 * length bytes)%nat.
+Proof.
+  (* TODO: bvector_eq is true iff the vectors are the same length *)
+Admitted.  
+
+Check bytes_bits_vector.
+Check HMAC_SHA256.HMAC.         (* ? *)
+Check HMAC.
+(* HMAC
+     : forall c p : nat,
+       (Bvector c -> Bvector (b c p) -> Bvector c) ->   // compression function h
+       Bvector c ->                          // iv, h's initialization vector
+       (Blist -> list (Bvector (b c p))) ->  // splitAndPad (e.g. generate_and_pad)
+       Bvector p ->                          // fpad, constant-length padding
+       Bvector (b c p) ->                    // opad
+       Bvector (b c p) ->                    // ipad
+
+^ Note: this has to do with the internals of SHA256 and HMAC too
+SHA's compression function, iv, generate_and_pad (with block vectors),
+HMAC's key padding function, HMAC's opad and ipad.
+How to convert?
+
+       Bvector (b c p) -> Blist -> Bvector c        // key, message, outputted hash
+
+k is of length b
+b = block size
+c = output size
+p = padding = b - c
+
+why pad the key? why not just let it be size b?
+ *)
+
+(* ----------------------------------------- Theorem and parameters *)
+
+(* want Bvector b = 512 bits *)
+Print Byte.int.
+Print Byte.repr.
+Check Byte.unsigned.
+Check HMAC_SHA256.sixtyfour.
+
+Definition opad_test := 
+     bytes_to_bits
+                     (map Byte.unsigned (HMAC_SHA256.sixtyfour (Byte.repr 52))).
+Check opad_test. 
+(* Definition ipad_test := bytes_to_bits
+                     (map Byte.unsigned (HMAC_SHA256.sixtyfour HMAC_SHA256.Ipad)). *)
+
+Check HMAC.
+
+(* ------------------------------------- *)
+Module Equiv.
+
+Definition c:nat := (SHA256_.DigestLength * 8)%nat.
+(*Variable p:nat.
+Locate HMAC.
+Check @HMAC. Check @sha_h.
+Check (@HMAC _ p (@sha_h _ p plus) sha_iv (sha_splitandpad_vector p) (fpad p)). 
+Check (HMAC (sha_h p plus) sha_iv).
+*)
+Definition p:=(32 * 8)%nat.
+
+Parameter sha_iv : Bvector (SHA256_.DigestLength * 8).
+
+(* Definition sha_h : list Z -> list Z := SHA256_.Hash. *)
+(* TODO: c = 32, p = 32 *)
+Parameter sha_h : Bvector c -> Bvector (c + p) -> Bvector c.
+
+(* corresponds to block size. b = plus *)
+
+(*  "Blist -> list (Bvector (b SHA256_.DigestLength c))" *)
+Parameter sha_splitandpad_vector :
+  Blist -> list (Bvector (SHA256_.DigestLength * 8 + p)).
+
+Parameter fpad : Bvector p.
+
+(* Define opad, define ipad, pass converted ipad/opad to respective hmacs *)
+
+(* Is this the theorem we want? Is it useful for the rest of the proofs?
+Should it be more abstract? *)
+
+(* TODO: opad <> ipad? *)
+(* TODO fill this in *)
+(* relies on bytes_bits_vector' too *)
+Parameter bytes_bits_conv_vector : byte -> Bvector (plus c p) -> Prop.
+(* Does something like: 
+bytes_bits_vector' (map Byte.unsigned (sixtyfour opad)) OPAD *)
+
+Locate sixtyfour.
+
+Definition bytes_bits_conv_vector'
+           (byte_pad : byte) (bits_pad : Bvector (c + p)) : bool :=
+  let bytes_pad := map Byte.unsigned (HMAC_SHA256.sixtyfour byte_pad) in
+  eqb (bytes_bits_vector_comp bytes_pad bits_pad) true.
+
+(* -------------- *)
+
+(*  (let (k_Out, k_In) :=
+                       splitVector (b 256 256) (b 256 256)
+                         (Vector.append (BVxor (b 256 256) K OP)
+                            (BVxor (b 256 256) K IP)) in 
+Possibly try n = m -> splitVector n m...
+*)
+
+SearchAbout Bvector.
+(* SearchAbout Vector. *)
+
+Lemma empty_vector : forall (v : Bvector 0),
+                       v = [].
+Proof.
+  intros v.
+  (* destruct v. *)
+
+Admitted.
+
+Lemma split_append_id : forall (len : nat) (v1 v2 : Bvector len),
+                          splitVector len len (Vector.append v1 v2) = (v1, v2).
+Proof.
+  induction len; intros v1 v2.
+  (* Case len = 0 *)
+    (* simpl. rewrite -> empty_vector. *)
+
+
+    Admitted.
+
+
+(* TODO: 10/25/14
+- figure out old and new fpad **
+- add lemma for xor **
+- fill in parameters: sha_h, sha_iv, sha_splitandpad_vector, fpad **
+- figure out how to get split lemmas to work
+- check bytes_bits_vector' fixpoint
+   - get it to eval
+   - see if induction works with it
+   - write bytes_bits_conv_vector X
+- step through theorem
+  - figure out how to use relations in theorem: compositional?
+
+ *)
+Theorem HMAC_spec_equiv : forall
+                            (k m h : list Z)
+                            (K : Bvector (plus c p)) (M : Blist) (H : Bvector c)
+                            (op ip : byte) (OP IP : Bvector (plus c p)),
+  ((length k) * 8)%nat = b c p ->
+  bytes_bits_vector_wrong k K ->
+  bytes_bits_lists m M ->
+  bytes_bits_conv_vector' op OP = true ->
+  bytes_bits_conv_vector' ip IP = true ->
+  HMAC sha_h sha_iv sha_splitandpad_vector fpad OP IP K M = H ->
+  HMAC_SHA256.HMAC op ip m k = h -> (* m k, not k m *)
+  bytes_bits_vector_comp h H = true.
+Proof.  
+  intros k m h K M H op ip OP IP.
+  intros padded_key_len padded_keys_eq msgs_eq ops_eq ips_eq.
+  intros HMAC_abstract HMAC_concrete.
+  unfold p,c, b in *.
+  simpl in *.
+
+  unfold HMAC in *.
+  unfold HMAC_SHA256.HMAC in *.
+
+  unfold HMAC_2K in *. unfold GHMAC_2K in *. (* unfold splitVector in *. *)
+  (* Still abstract: sha_h, sha_splitandpad_vector, fpad,
+     bytes_bits_vector', bytes_bits_conv_vector *)
+  rewrite -> split_append_id in HMAC_abstract. 
+
+  unfold HMAC_SHA256.OUTER in *. unfold HMAC_SHA256.INNER in *.
+    unfold HMAC_SHA256.outerArg in *. unfold HMAC_SHA256.innerArg in *.
+    unfold HMAC_SHA256.mkArgZ in *. unfold HMAC_SHA256.mkArg in *.
+
+  unfold BVxor in *. unfold xorb in *. (* unfold Vector.map2 in *. *)
+  unfold Byte.xor in *. (* unfold Z.lxor in *. *)
+
+    (* Lemma:
+
+BVxor (b 256 256) K OP = Vector.map2 xorb K OP (can unfold xorb) 
+     ~
+                          (map
+                          (fun p0 : byte * byte => Byte.xor (fst p0) (snd p0))
+                          (combine (map Byte.repr (HMAC_SHA256.mkKey k))
+                             (HMAC_SHA256.sixtyfour ip)))
+
+probably want a meta-lemma for composition of relations
+r1 x X -> r2 y Y -> f x y ~ F X Y
+
+figure out how to approach proof: avoid 4-way induction
+ *)
+
+    
+  rewrite <- HMAC_abstract.
+  rewrite <- HMAC_concrete.
+
+  
+  
+  induction msgs_eq.
+
+
+Abort.
+=======
+Set Implicit Arguments.
+
+Require Import Bvector.
+Require Import List.
+Require Import Arith.
+
+Require Import HMAC_functional_prog.
+Require Import Integers.
+Require Import Coqlib.
+
+(* Require Import List. Import ListNotations. *)
+
+Definition Blist := list bool.
+
+Fixpoint splitVector (A : Set) (n m : nat) :
+  Vector.t A (n + m) -> (Vector.t A n * Vector.t A m) :=
+  match n with
+    | 0%nat => 
+      fun (v : Vector.t A (O + m)) => (@Vector.nil A, v) (* why the function? TODO *)
+    | S n' => 
+      fun (v : Vector.t A (S n' + m)) => 
+        let (v1, v2) := splitVector _ _ (Vector.tl v) in
+          (Vector.cons _ (Vector.hd v) _ v1, v2)
+  end.
+
+Eval compute in splitVector 1 2 [true; true; true].
+
+Section HMAC.
+
+SearchAbout Bvector.
+Print Bvector.
+Check Bvector 10.
+Check [true]. 
+Print Vector.
+
+(* b = block size
+   c = digest (output) size
+   p = padding = b - c (fixed) *)
+  Variable c p : nat.
+  Definition b := (c + p)%nat.
+  
+  (* The compression function *)
+  Variable h : Bvector c -> Bvector b -> Bvector c.
+  (* The initialization vector is part of the spec of the hash function. *)
+  Variable iv : Bvector c.
+  (* The iteration of the compression function gives a keyed hash function on lists of words. *)
+  Definition h_star k (m : list (Bvector b)) :=
+    fold_left h m k.
+  (* The composition of the keyed hash function with the IV gives a hash function on lists of words. *)
+  Definition hash_words := h_star iv.
+
+  (* TODO check how this corresponds to SHA
+     Seems that h = SHA compression function
+     hash_words with SHA's iv is SHA
+   *)
+  Check hash_words.
+  Check h_star.
+
+  Variable splitAndPad : Blist -> list (Bvector b).
+
+  (* TODO examine this hypothesis, prove that MD lemmas imply it *)
+  Hypothesis splitAndPad_1_1 : 
+    forall b1 b2,
+      splitAndPad b1 = splitAndPad b2 ->
+      b1 = b2.
+  
+  (* constant-length padding. *)
+  Variable fpad : Bvector p.
+
+  Definition app_fpad (x : Bvector c) : Bvector b :=
+    (Vector.append x fpad).
+  Definition h_star_pad k x :=
+    app_fpad (h_star k x).
+
+  Definition GNMAC k m :=
+    let (k_Out, k_In) := splitVector c c k in
+    h k_Out (app_fpad (h_star k_In m)).
+
+  (* The "two-key" version of GHMAC and HMAC. *)
+  (* Concatenate (K xor opad) and (K xor ipad) *)
+  Definition GHMAC_2K (k : Bvector (b + b)) m :=
+    let (k_Out, k_In) := splitVector b b k in (* concat earlier, then split *)
+      let h_in := (hash_words (k_In :: m)) in 
+        hash_words (k_Out :: (app_fpad h_in) :: nil).
+  
+  Definition HMAC_2K (k : Bvector (b + b)) (m : Blist) :=
+    GHMAC_2K k (splitAndPad m).
+
+Check HMAC_2K.
+(* HMAC_2K
+     : Bvector (b + b) -> Blist -> Bvector c *)
+
+(* opad and ipad are constants defined in the HMAC spec. *)
+Variable opad ipad : Bvector b.
+Definition GHMAC (k : Bvector b) :=
+  GHMAC_2K (Vector.append (BVxor _ k opad) (BVxor _ k ipad)).
+
+Print BVxor.
+
+
+Definition HMAC (k : Bvector b) :=
+  HMAC_2K (Vector.append (BVxor _ k opad) (BVxor _ k ipad)).
+
+Check HMAC.                     (*  : Bvector b -> Blist -> Bvector c *)
+
+End HMAC.
+
+(* ----------------------------------------------------------- Theorem definitions *)
+
+Check HMAC_SHA256.HMAC.            (* list Z -> list Z -> list Z *)
+
+  (* Bvector is little-endian (least significant bit at head; list Z are just translated
+from the string (ascii -> nat -> Z); but Int are packed big-endian (with 4 Z -> 1 Int)
+
+each Z is one byte (8 bits) *)
+
+(* TODO: add isbyteZ (from SHA256.v), 0 <= i <= 256 *)
+
+(* *************** byte/bit computational *)
+
+(* TODO: finish this
+
+The term "Vector.append (iterate n' num_new) [bool_digit]" has type
+ "Vector.t bool (n' + 1)" while it is expected to have type 
+"Bvector (S n')".
+
+Function with proof of equivalence? see hash_blocks  *)
+
+(*
+Fixpoint iterate (n : nat) (byte : nat) : Bvector n :=
+  match n as x return Bvector x with
+    | O => Vector.nil bool
+    | S n' =>
+      let byte_subtract := (byte - NPeano.pow 2 n')%nat in
+      let bool_digit := negb (leb byte_subtract 0) in
+      let num_new := if bool_digit then byte_subtract else byte in
+      Vector.append (iterate n' num_new) [bool_digit] (* could reverse instead *)
+  end.
+
+*)
+
+Lemma add_1_r_S : forall (n : nat), (n + 1)%nat = S n.
+Proof.
+  induction n.
+    reflexivity.
+    simpl. rewrite -> IHn. reflexivity.
+Defined.
+
+(* TODO step through this *)
+Locate leb. Check negb.
+(* little-endian *)
+Fixpoint iterate (n : nat) (byte : nat) : Bvector n.
+Proof.
+  destruct n.
+     apply (Vector.nil bool).
+  remember ((byte - NPeano.pow 2 n)%nat) as byte_subtract.
+  remember (negb (leb byte_subtract 0)) as bool_digit. (* changed from leb: gt now *)
+  remember (if bool_digit then byte_subtract else byte) as num_new.
+  rewrite <- add_1_r_S.
+  apply (Vector.append (iterate n num_new) [bool_digit]). (* n' *)
+Defined.
+
+Print iterate.
+Eval compute in iterate 1 255.
+Check eq_rec. Print eq_rec. Print eq_rect. Check eq_rect.
+Print NPeano.Nat.add_1_r.
+
+(* TODO: fix the latter + 1 *)
+Fixpoint byte_to_bits (byte : Z) : Bvector 8 :=
+  let max_pow_two := 7%nat in
+  iterate (max_pow_two + 1) (nat_of_Z byte + 1).
+
+  Print add_1_r_S.
+Eval compute in iterate 8 2.
+Eval compute in byte_to_bits 0.
+Eval compute in byte_to_bits 1.
+Eval compute in byte_to_bits 2.
+
+Eval compute in byte_to_bits 127.
+Eval compute in byte_to_bits 128.
+Eval compute in byte_to_bits 129.
+Eval compute in byte_to_bits 200.
+Eval compute in byte_to_bits 255. 
+Eval compute in byte_to_bits 256. (* not valid *)
+
+(* Parameter byte_to_bits : Z -> Bvector 8. *)
+
+(* Or: concatMap byte_to_bit bytes *)
+Check Bvector.
+SearchAbout Bvector.
+Print Vector.t.
+
+(* how to prove that it's length bytes * 8? *)
+(* list of bytes? (type) *)
+Fixpoint bytes_to_bits (bytes : list Z) : Bvector (length bytes * 8) :=
+  match bytes as x return Bvector (length x * 8) with (* CPDT *)
+    | nil => Vector.nil bool
+    | x :: xs => Vector.append (byte_to_bits x) (bytes_to_bits xs)
+  end.
+
+
+
+(* ************* inductive defs *)
+  
+SearchAbout Bvector.
+
+Definition asZ (x : bool) : Z := if x then 1 else 0.
+
+(* TODO: maybe prefer b : byte, with Byte.repr? *)
+Definition convertByteBits (b : Z) (B : Bvector 8) : Prop :=
+  exists (b0 b1 b2 b3 b4 b5 b6 b7 : bool),
+   B = [b0; b1; b2; b3; b4; b5; b6; b7] /\
+   b =  (1 * (asZ b0) + 2 * (asZ b1) + 4 * (asZ b2) + 8 * (asZ b3)
+         + 16 * (asZ b4) + 32 * (asZ b5) + 64 * (asZ b6) + 128 * (asZ b7)).
+
+(* *** *)
+
+(* relationship between a list Z (of bytes) and a Bvector of size (c + p):
+toBvector (bytes_to_bits k) = K?
+
+This definition is not easy to use; replaced with bytes_bits_vector' in theorem
+ *)
+Inductive bytes_bits_vector (c p : nat) (k : list Z) : Bvector (plus c p) -> Prop :=
+  | test_n : forall (K : Bvector (plus c p)),
+               bytes_bits_vector c p k K (* TODO *)
+.
+
+(* relating list Z to Blist
+bytes_to_bits m = length M
+
+TODO: big-endian, little-endian?
+*)
+Inductive bytes_bits_lists : list Z -> Blist -> Prop :=
+  | eq_empty : bytes_bits_lists nil nil
+  | eq_cons : forall (bytes : list Z) (bits : Blist)
+                     (byte : Z) (b0 b1 b2 b3 b4 b5 b6 b7 : bool),
+                bytes_bits_lists bytes bits ->
+                convertByteBits byte [b0; b1; b2; b3; b4; b5; b6; b7] ->
+                bytes_bits_lists (byte :: bytes)
+                                (b0 :: b1 :: b2 :: b3 :: b4 :: b5 :: b6 :: b7 :: bits)
+.
+
+(* the hashes are "the same": list Z vs Bvector c
+
+toBvector (bytes_to_bits h) = H
+this is *almost* the same as bytes_bits_vector, except just c, not c + p
+ *)
+(* note: need to name c in order to use in Bvector c -- but then need to use names *)
+Inductive bytes_bits_vector_wrong (len : nat) (bytes : list Z) (bits : Bvector len) : Prop :=
+  | eq_empty_v' : bytes = nil -> len = 0%nat -> bytes_bits_vector_wrong bytes bits
+  | eq_cons_v' : bytes_bits_vector_wrong bytes bits.
+
+(*
+Fixpoint iterate (n : nat) (byte : nat) : Bvector n.
+Proof.
+  destruct n.
+     apply (Vector.nil bool).
+  remember ((byte - NPeano.pow 2 n)%nat) as byte_subtract.
+  remember (negb (leb byte_subtract 0)) as bool_digit. (* changed from leb: gt now *)
+  remember (if bool_digit then byte_subtract else byte) as num_new.
+  rewrite <- add_1_r_S.
+  apply (Vector.append (iterate n num_new) [bool_digit]). (* n' *)
+Defined.
+*)
+
 (*
 Inductive bytes_bits_vector' (l : list Z) : Bvector (8 * length l) -> Prop :=
   | eq_empty_v : forall (bits : Bvector (8 * length nil)),
